IMLTT/JudgmentsAndRules.lean
@@ -28,8 +28,10 @@ mutual
                    → IsType Γ (Tm.sigma A B)
     | iden_form : IsType Γ A
                   → IsType ((Γ ⬝ A) ⬝ (lift 0 1 A)) (Tm.iden A 1 0)
-    | univ_form : IsType Γ U
-    | univ_elim : HasType Γ A U → IsType Γ A
+    | univ_form : IsCtx Γ
+                  → IsType Γ U
+    | univ_elim : HasType Γ A U
+                  → IsType Γ A
 
   -- Γ ⊢ a : A
   inductive HasType : Ctx → Tm → Tm → Prop where
@@ -47,32 +49,33 @@ mutual
     | sigma_intro : HasType Γ a A → HasType Γ b (substitute B a 0)
                     → HasType Γ (Tm.pairSigma a b) (Tm.sigma A B)
     | iden_intro : IsType Γ A
-                   → HasType (Γ ⬝ A) (Tm.refl 0) (Tm.iden A 0 0)
+                   → HasType (Γ ⬝ A) (Tm.refl A 0) (Tm.iden A 0 0)
     -- universe intro
     | univ_unit : IsCtx Γ
                   → HasType Γ 𝟙 U
-    | univ_empty : IsCtx Γ →
-                   HasType Γ 𝟘 U
+    | univ_empty : IsCtx Γ
+                   → HasType Γ 𝟘 U
     | univ_pi : HasType Γ A U → HasType (Γ ⬝ A) B U
                 → HasType Γ (Tm.pi A B) U
     | univ_sigma : HasType Γ A U → HasType (Γ ⬝ A) B U
-                 → HasType Γ (Tm.sigma A B) U
+                   → HasType Γ (Tm.sigma A B) U
     | univ_iden : HasType Γ A U
                   → HasType ((Γ ⬝ A) ⬝ (lift 0 1 A)) (Tm.iden A 0 1) U
     -- elimination rules (except univ)
-    | unit_elim : IsType (Γ ⬝ Tm.unit) C → HasType Γ c (substitute C Tm.unit 0) → HasType Γ p Tm.unit
-                  → HasType Γ (Tm.indUnit p c) (substitute C p 0)
+    | unit_elim : IsType (Γ ⬝ Tm.unit) C → HasType Γ c (substitute C Tm.unit 0)
+                  → HasType Γ p Tm.unit
+                  → HasType Γ (Tm.indUnit C p c) (substitute C p 0)
     | empty_elim : IsType (Γ ⬝ 𝟘) C → HasType Γ p 𝟘
-                   → HasType Γ (Tm.indEmpty p) (substitute C p 0)
+                   → HasType Γ (Tm.indEmpty C p) (substitute C p 0)
     | pi_elim : HasType Γ f (Tm.pi A B) → HasType Γ a A
                 → HasType Γ (Tm.app f a) (substitute B a 0)
     | sigma_elim : HasType Γ p (Tm.sigma A B) → IsType (Γ ⬝ (Tm.sigma A B)) C
                    → HasType (Γ ⬝ A ⬝ B) c (substitute C (Tm.pairSigma 1 0) 0)
-                   → HasType Γ (Tm.indSigma c p) (substitute C p 0)
+                   → HasType Γ (Tm.indSigma A B C c p) (substitute C p 0)
     | iden_elim : IsType (((Γ ⬝ A) ⬝ (lift 0 1 A)) ⬝ (Tm.iden A a b)) C
                   → HasType (Γ ⬝ A) t
-                      (substitute (substitute (substitute C 0 2) 0 1) (Tm.refl 0) 0)
-                  → HasType (((Γ ⬝ A) ⬝ (lift 0 1 A)) ⬝ (Tm.iden A 2 1)) (Tm.j t 2 1 0) C
+                    (substitute (substitute (substitute C 0 2) 0 1) (Tm.refl A 0) 0)
+                  → HasType (((Γ ⬝ A) ⬝ (lift 0 1 A)) ⬝ (Tm.iden A 2 1)) (Tm.j A t 2 1 0) C
     -- conversion
     | ty_conv : IsType Γ A → IsType Γ B → HasType Γ a A → IsEqualType Γ A B
                 → HasType Γ a B
@@ -80,39 +83,45 @@ mutual
   -- Γ ⊢ A ≡ B type
   inductive IsEqualType : Ctx → Tm → Tm → Prop where
     -- congruence rules (formation)
-    | unit_form_eq : IsCtx Γ → IsEqualType Γ Tm.unit Tm.unit
-    | empty_form_eq : IsCtx Γ → IsEqualType Γ Tm.empty Tm.empty
+    | unit_form_eq : IsCtx Γ
+                     → IsEqualType Γ Tm.unit Tm.unit
+    | empty_form_eq : IsCtx Γ
+                      → IsEqualType Γ Tm.empty Tm.empty
     | pi_form_eq : IsEqualType Γ A A' → IsEqualType (Γ ⬝ A) B B'
                    → IsEqualType Γ (Tm.pi A B) (Tm.pi A' B')
     | sigma_form_eq : IsEqualType Γ A A' → IsEqualType (Γ ⬝ A) B B'
                       → IsEqualType Γ (Tm.sigma A B) (Tm.sigma A' B')
-    | iden_form_eq : IsEqualType Γ A A' → IsEqualType (Γ ⬝ A ⬝ (lift 0 1 A)) (Tm.iden A 1 0) (Tm.iden A 1 0)
-    | univ_form_eq : IsCtx Γ → IsEqualType Γ Tm.univ Tm.univ
+    | iden_form_eq : IsEqualType Γ A A'
+                     → IsEqualType (Γ ⬝ A ⬝ (lift 0 1 A)) (Tm.iden A 1 0) (Tm.iden A 1 0)
+    | univ_form_eq : IsCtx Γ
+                     → IsEqualType Γ Tm.univ Tm.univ
     | univ_elim_eq : IsEqualTerm Γ A A' Tm.univ → IsEqualType Γ A A'
 
   -- Γ ⊢ a ≡ b : A
   inductive IsEqualTerm : Ctx → Tm → Tm → Tm → Prop where
     -- computation rules
     | unit_comp : IsType (Γ ⬝ 𝟙) C → HasType Γ c (substitute C Tm.tt 0)
-                  → IsEqualTerm Γ (Tm.indUnit Tm.tt c) Tm.tt (substitute C Tm.tt 0)
+                  → IsEqualTerm Γ (Tm.indUnit A Tm.tt c) Tm.tt (substitute C Tm.tt 0)
     | pi_comp : HasType (Γ ⬝ A) b B → HasType Γ a A
                 → IsEqualTerm Γ (Tm.app (Tm.lam A b) a) (substitute b a 0) (substitute B a 0)
     | sigma_comp : HasType Γ a A → HasType (Γ ⬝ A) b (substitute B a 0)
                    → IsType (Γ ⬝ (Tm.sigma A B)) C
                    → HasType (Γ ⬝ A ⬝ B) c (substitute C (Tm.pairSigma 1 0) 0)
-                   → IsEqualTerm Γ (Tm.indSigma c (Tm.pairSigma a b)) (substitute (substitute c a 0) b 0)
-                     (substitute C (Tm.pairSigma a b) 0)
+                   → IsEqualTerm Γ (Tm.indSigma A B C c (Tm.pairSigma a b))
+                     (substitute (substitute c a 0) b 0) (substitute C (Tm.pairSigma a b) 0)
     | iden_comp : IsType (((Γ ⬝ A) ⬝ (lift 0 1 A)) ⬝ (Tm.iden A a b)) C
-                  → HasType (Γ ⬝ A) t (substitute (substitute (substitute C 0 2) 0 1) (Tm.refl 0) 0)
-                  → IsEqualTerm (Γ ⬝ A) (Tm.j t 0 0 (Tm.refl 0)) t
-                      (substitute (substitute (substitute C 0 2) 0 1) (Tm.refl 0) 0)
+                  → HasType (Γ ⬝ A) t
+                    (substitute (substitute (substitute C 0 2) 0 1) (Tm.refl A 0) 0)
+                  → IsEqualTerm (Γ ⬝ A) (Tm.j A t 0 0 (Tm.refl A 0)) t
+                      (substitute (substitute (substitute C 0 2) 0 1) (Tm.refl A 0) 0)
     -- congruence rules (introduction and elimination)
-    | unit_intro_eq : IsCtx Γ → IsEqualTerm Γ Tm.tt Tm.tt Tm.unit
+    | unit_intro_eq : IsCtx Γ
+                      → IsEqualTerm Γ Tm.tt Tm.tt Tm.unit
     | unit_elim_eq : IsEqualType (Γ ⬝ 𝟙) A A' → IsEqualTerm Γ a a' (substitute A Tm.tt 0)
                      → IsEqualTerm Γ b b' Tm.unit
-                     → IsEqualTerm Γ (Tm.indUnit b a) (Tm.indUnit b' a') (substitute A b 0)
+                     → IsEqualTerm Γ (Tm.indUnit A b a) (Tm.indUnit A' b' a') (substitute A b 0)
     | empty_elim_eq : IsEqualType (Γ ⬝ Tm.empty) A A' → IsEqualTerm Γ b b' Tm.empty
-                      → IsEqualTerm Γ (Tm.indEmpty b) (Tm.indEmpty b') (substitute A b 0)
+                      → IsEqualTerm Γ (Tm.indEmpty A b) (Tm.indEmpty A' b') (substitute A b 0)
     | pi_intro_eq : IsEqualType Γ A A' → IsEqualType (Γ ⬝ A) B B' → IsEqualTerm (Γ ⬝ A) b b' B
                     → IsEqualTerm Γ (Tm.lam A b) (Tm.lam A' b') (Tm.pi A B)
     | pi_elim_eq : IsEqualType Γ (Tm.pi A B) (Tm.pi A' B') → IsEqualTerm Γ a a' A
@@ -123,12 +132,12 @@ mutual
     | sigma_elim_eq : IsEqualType Γ (Tm.sigma A B) (Tm.sigma A' B')
                       → IsEqualTerm Γ p p' (Tm.sigma A B) → IsEqualType (Γ ⬝ (Tm.sigma A B)) C C'
                       → IsEqualTerm (Γ ⬝ A ⬝ B) c c' (substitute C (Tm.pairSigma 1 0) 0)
-                      → IsEqualTerm Γ (Tm.indSigma c p) (Tm.indSigma c' p') (substitute C p 0)
-    | iden_intro_eq : IsEqualType Γ A A' → IsEqualTerm (Γ ⬝ A) (Tm.refl 0) (Tm.refl 0) (Tm.iden A 0 0)
+                      → IsEqualTerm Γ (Tm.indSigma A B C c p) (Tm.indSigma A B C c' p') (substitute C p 0)
+    | iden_intro_eq : IsEqualType Γ A A' → IsEqualTerm (Γ ⬝ A) (Tm.refl A 0) (Tm.refl A 0) (Tm.iden A 0 0)
     | iden_elim_eq : IsEqualType Γ A A' → IsEqualType (Γ ⬝ A ⬝ A ⬝ (Tm.iden A 1 0)) B B'
                      → IsEqualTerm (Γ ⬝ A) b b'
-                       (substitute (substitute (substitute B 0 1) 0 2) (Tm.refl 0) 0)
-                     → IsEqualTerm (Γ ⬝ A ⬝ A ⬝ (Tm.iden A 1 0)) (Tm.j b 2 1 0) (Tm.j b 2 1 0) B
+                       (substitute (substitute (substitute B 0 1) 0 2) (Tm.refl A 0) 0)
+                     → IsEqualTerm (Γ ⬝ A ⬝ A ⬝ (Tm.iden A 1 0)) (Tm.j A b 2 1 0) (Tm.j A b 2 1 0) B
     -- conversion
     | ty_conv_eq : IsType Γ A → IsType Γ B → HasType Γ a A → HasType Γ b B 
                    → IsEqualTerm Γ a b A → IsEqualType Γ A B
@@ -142,11 +151,13 @@ notation Γ " ⊢ " A " ≡ " B => IsEqualType Γ A B
 notation Γ " ⊢ " s " ≡ " t " ∶ " A => IsEqualTerm Γ s t A
 
 
--- testing
+axiom eq : substitute (Tm.pi 2 1) 1 0 = Tm.pi 2 1
 
+-- testing
 example (hA : IsType (Ctx.empty ⬝ 𝟙 ⬝ 𝟘 ⬝ 𝟙) (Tm.pi 2 1))
         (haA : HasType (Ctx.empty ⬝ 𝟙 ⬝ 𝟘) a (Tm.pi 2 1))
         (hbU : HasType (Ctx.empty ⬝ 𝟙 ⬝ 𝟘) Tm.tt Tm.unit):
-  HasType (Ctx.empty ⬝ 𝟙 ⬝ 𝟘) (Tm.indUnit Tm.tt a) (Tm.pi 2 1) :=
-    HasType.unit_elim hA haA hbU
-
+  HasType (Ctx.empty ⬝ 𝟙 ⬝ 𝟘) (Tm.indUnit A Tm.tt a) (Tm.pi 2 1) :=
+    by
+      apply HasType.unit_elim hA haA hbU
+      rw [eq]
